\documentclass[12pt]{article}
\usepackage{fullpage,enumitem,amsmath,amssymb,graphicx}

\begin{document}

\begin{center}
{\Large CSED342 Assignment 8 \vspace{10pt}}

\begin{tabular}{rl}
Student ID: & 20220140 \\
Name: & Taeyeon Kim \\
\end{tabular}
\end{center}

\begin{center}
By turning in this assignment, I agree by the POSTECH honor code and declare that all of this is my own work.
\end{center}

\section*{Problem 2a}

First, our knowledge $KB$ base is constructed of
\[
KB = \{(A \lor B) \implies \lnot C, \lnot (\lnot A \lor C) \implies D, A \}
\]

Convert each knowledge in $KB$ into CNF with using $\frac{P \implies Q}{\lnot P \lor Q}$, therefore we earn
\[
KB = \{(A \lor B) \implies \lnot C, \lnot A \lor C \lor D, A \}
\]

Rewrite using $\frac{\lnot P \lor Q}{P \implies Q}$,
\[
KB = \{(A \lor B) \implies \lnot C, A \implies (C \lor D), A \}
\]

Apply Modus Ponens to $A \implies (C \lor D)$ with $A$,
\[
KB = \{(A \lor B) \implies \lnot C, (C \lor D), A \}
\]

Apply Modus Ponens to $(A \lor B) \implies \lnot C$ with $A$,
\[
KB = \{\lnot C, (C \lor D), A \}
\]

\because $A \in KB$, $A$ is always true, therefore disjuction with any variable would return true.


Finally $\lnot C \in KB$ and $C \land D \in KB$, $C$ is always false. However by $C \lor D$, at least one of $C$ or $D$ must be true.
Therefore $D$ is true, \textbf{D} satisfies.

\null\hfill\square


\section*{Problem 2b}


Given knowledge base is following
\[
KB = \{A \lor B, B \implies C, (A \lor C) \implies D \}
\]

Convert $B \implies C$ into CNF.

\[
KB = \{A \lor B, \lnot B \lor C, (A \lor C) \implies D \}
\]

Convert $(A \lor C) \implies D$ into CNF.
\[
KB = \{A \lor B, \lnot B \lor C, \lnot (A \lor C) \lor D \}
\]

Apply De Morgan's law into $\lnot (A \lor C) \lor D$.
\[
KB = \{A \lor B, \lnot B \lor C, (\lnot A \land \lnot C) \lor D \}
\]

Apply Distributive law into $(\lnot A \land \lnot C) \lor D$.
\[
KB = \{A \lor B, \lnot B \lor C, (\lnot A \lor D) \land (\lnot C \lor D) \}
\]

Split $(\lnot A \lor D) \land (\lnot C \lor D)$ into 2 constraints.
\[
KB = \{A \lor B, \lnot B \lor C, \lnot A \lor D, \lnot C \lor D \}
\]

Use resolution rule with $A \lor B$ and $\lnot B \lor C$.
\[
KB = \{A \lor C, \lnot A \lor D, \lnot C \lor D \}
\]

Use resolution rule with $A \lor C$ and $\lnot C \lor D$.
\[
KB = \{\lnot A \lor D, A \lor D \}
\]

Use resolution rule with $\lnot A \lor D$ and $A \lor D$.
\[
KB = \{ D \}
\]

Therefore $D$ is true, \textbf{D} satisfies. \\
\null\hfill\square
\end{document}
